theories/DirtyBootstrap.v
@@ -1,0 +1,92 @@
+From LibTx Require Import
+     Storage
+     Handlers.Deterministic
+     SLOT.
+
+From Coq Require Import
+     List.
+Import ListNotations.
+
+Section defn.
+  Context K V DB `{@Storage K V DB}.
+
+  (* We have only two processes in the system: [writer] that creates
+  local transactions and [agent] that is used to bootstrap the remote
+  replica: *)
+  Inductive Pid := writer | agent.
+
+  Definition Handler := KV.t Pid DB
+                    <+> Log.t Pid (@Wlog_elem K V).
+
+  Section boilerplate.
+    Definition req_t := get_handler_req_pid Handler.
+    Definition ret_t := get_handler_ret_pid Handler.
+
+    Definition read (k : K) : req_t.
+      lift (@KV.read K V k).
+    Defined.
+
+    Definition keys : req_t.
+      lift (@KV.keys K V).
+    Defined.
+
+    Definition write (k : K) (v : V) : req_t.
+      lift (KV.write k v).
+    Defined.
+
+    Definition delete (k : K) : req_t.
+      lift (@KV.delete K V k).
+    Defined.
+
+    Definition forward_op (w : @Wlog_elem K V) : req_t.
+      lift (fun (_ : Pid) => w).
+    Defined.
+  End boilerplate.
+
+  Definition wlog_apply (w : @Wlog_elem K V) :=
+    match w with
+    | wl_write k v => write k v
+    | wl_delete k => delete k
+    end.
+
+  Let Thread := @Thread req_t ret_t.
+
+  Fixpoint writer_loop (ops : @Wlog K V) : Thread :=
+    match ops with
+    | [] => t_dead
+    | op :: tail =>
+      do _ <- wlog_apply op;
+      writer_loop tail
+    end.
+
+  Fixpoint bootstrap (keys : list K) cont : Thread :=
+    match keys with
+    | [] => cont I
+    | k :: tail =>
+      do ret <- read k;
+      match ret with
+      | Some v =>
+        do _ <- forward_op (wl_write k v);
+        bootstrap tail cont
+      | None =>
+        bootstrap tail cont
+      end
+    end.
+
+  Fixpoint export_wlog (ops : @Wlog K V) cont : Thread :=
+    match ops with
+    | [] => cont I
+    | op :: tail =>
+      do _ <- forward_op op;
+      export_wlog tail cont
+    end.
+
+  Definition exporter (ops : @Wlog K V) : Thread :=
+    do kk <- keys;
+    call _ <- bootstrap kk;
+    call _ <- export_wlog ops;
+    t_dead.
+
+  Definition dirty_bootstrapper ops := (ThreadGenerator writer (writer_loop ops))
+                                   -|| (ThreadGenerator agent (exporter ops)).
+End defn.
